aneris/examples/crdt/statelib/proof/stlib_proof_utils.v
@@ -1,0 +1,168 @@
+From stdpp Require Import gmap.
+
+From iris.base_logic Require Import invariants bi.
+From iris.algebra Require Import agree auth excl gmap.
+
+From aneris.algebra Require Import monotone.
+From aneris.aneris_lang
+  Require Import lang network tactics proofmode lifting resources.
+From aneris.aneris_lang.lib
+  Require Import list_proof lock_proof vector_clock_proof serialization_proof
+    map_proof lock_proof network_util_proof inject.
+From aneris.aneris_lang.lib.serialization Require Import serialization_proof.
+From aneris.aneris_lang.lib.vector_clock Require Import vector_clock_proof.
+From aneris.aneris_lang.program_logic Require Import lightweight_atomic.
+From aneris.prelude Require Import misc time.
+
+From aneris.examples.crdt.spec
+  Require Import crdt_events crdt_resources crdt_denot crdt_time crdt_base.
+From aneris.examples.crdt.statelib.resources
+  Require Import resources resources_inv resources_local resources_global resources_lock.
+
+From aneris.examples.crdt.statelib Require Import statelib_code.
+From aneris.examples.crdt.statelib.user_model
+  Require Import params model semi_join_lattices.
+From aneris.examples.crdt.statelib.time Require Import time.
+From aneris.examples.crdt.statelib.STS Require Import utils gst lst.
+From aneris.examples.crdt.statelib.proof
+  Require Import spec events resources utils resources.
+
+Instance timeinst : Log_Time := timestamp_time.
+
+Ltac token_excl A B := (try (iDestruct (own_valid_2 with A) as %B; destruct B)).
+
+
+(** Nomenclature:
+  * In this file (in every section) there are physical and logical operations
+  * and states. I will try to use the following names to help reading the proofs
+  * and specifications.
+  *
+  *  → Operations:
+  *    ↪ in AnerisLang      (type: val)  : op_v
+  *    ↪ logical operations (type LogOp) : op_log
+  *
+  *  → States:
+  *    ↪ serialized         (type: val)  : st_serialized
+  *    ↪ in AnerisLang      (type: val)  : st_v
+  *    ↪ logical operations (type LogSt) : st_log
+  *    ↪ local states, STS  (type Lst) : lst
+  *    ↪ global states, STS (type Gst) : lst
+  *
+  * Note on coherence:
+  *
+  * There are coherence predicates over these different versions of operations
+  * and states:
+  *
+  * → Operations:
+  *    ↪ LogOp → val : StLib_Op_Coh
+  *
+  * → States:
+  *    ↪ val   ↔ serialized : StLib_StSerialization
+  *    ↪ LogSt → val        : StLib_St_Coh
+  *    ↪ Lst   → LogSt      : denotation
+  *
+  *)
+
+
+
+Section ToBeMoved.
+  Context `{!anerisG Mdl Σ}.
+
+  (** TODO: factorize loop_forever and this spec.
+    * The following has been copied from
+    * [aneris/examples/rcb/proof/proof_of_network.v] *)
+  Lemma wp_loop_forever (fv : val) P ip :
+    {{{ {{{ P }}} fv #() @[ip] {{{ RET #(); P }}} ∗
+        P
+    }}}
+      loop_forever fv @[ip]
+    {{{ RET #(); False }}}.
+  Proof.
+    iIntros (ϕ) "[#Hfv HP] Hϕ".
+    iLöb as "IH".
+    rewrite /loop_forever.
+    wp_pures.
+    wp_bind (fv _).
+    iApply ("Hfv" with "HP").
+    iModIntro.
+    iIntros "HP". do 2 wp_pure _.
+    iApply ("IH" with "HP").
+    done.
+  Qed.
+
+End ToBeMoved.
+
+Section ToBeMoved'.
+
+  Context `{!anerisG Mdl Σ, !EqDecision LogOp, !Countable LogOp,
+            !CRDT_Params, !Lattice LogSt, !StLib_Params LogOp LogSt}.
+
+  Notation StLib_Serializable v := (Serializable StLib_StSerialization v).
+  Record StLib_SerializableVal :=
+    StLib_SerVal {StLib_SV_val : val;
+            StLib_SV_ser : StLib_Serializable StLib_SV_val }.
+  Coercion StLib_SV_val : StLib_SerializableVal >-> val.
+  Existing Instance StLib_SV_ser.
+  Arguments StLib_SerVal _ {_}.
+
+End ToBeMoved'.
+
+
+
+Section SocketProtolDefinition.
+
+  Context {LogOp LogSt : Type}.
+  Context `{!anerisG Mdl Σ, !EqDecision LogOp, !Countable LogOp,
+            !CRDT_Params, !Lattice LogSt, !StLib_Params LogOp LogSt}.
+  Context `{!Internal_StLibG LogOp Σ, !StLib_GhostNames}.
+
+  Definition socket_proto (repId : RepId) : socket_interp Σ :=
+    λ m,
+      let (from, to) := (m_sender m, m_destination m) in
+      let mb := m_body m in
+      (∃ (st_v: val) (st_log: LogSt) (h__local h__sub: event_set LogOp),
+        ⌜ s_is_ser StLib_StSerialization st_v mb ⌝ ∗
+        ⌜ StLib_St_Coh st_log st_v ⌝ ∗
+        ⌜⟦h__local ∪ h__sub⟧ ⇝ st_log⌝ ∗
+        StLib_OwnLocalSnap repId h__local h__sub)%I.
+
+  Global Instance socket_proto_Persistent (repId: RepId) (m: message):
+    Persistent (socket_proto repId m).
+  Proof. apply _. Qed.
+
+  Definition socket_inv (repId: RepId) (h: socket_handle) (z: socket_address) (s: socket) : iProp Σ :=
+    inv (nroot .@ "socketinv")
+      (∃ R S,
+        h ↪[ip_of_address z] s ∗
+        ⌜ saddress s = Some z ⌝ ∗
+        ⌜ CRDT_Addresses !! repId = Some z ⌝ ∗
+        z ⤳ (R, S) ∗
+        [∗ set] m ∈ R, socket_proto repId m).
+
+End SocketProtolDefinition.
+
+
+
+Section LockInvariant.
+
+  Context {LogOp LogSt : Type}.
+  Context `{!anerisG Mdl Σ, !EqDecision LogOp, !Countable LogOp,
+            !CRDT_Params, !Lattice LogSt, !StLib_Params LogOp LogSt}.
+  Context `{!Internal_StLibG LogOp Σ, !StLib_GhostNames}.
+
+  Definition lock_inv_aux (i : RepId) (st_loc : loc) : iProp Σ :=
+    ∃ (ip : ip_address) (phys_st : val) (log_st : LogSt)
+      (h__own h__for : gset (Event LogOp)),
+      ⌜ip_of_address <$> CRDT_Addresses !! i = Some ip⌝ ∗
+     st_loc ↦[ip] phys_st ∗
+      ⌜StLib_St_Coh log_st phys_st⌝ ∗
+      OwnLockInv i h__own h__for ∗
+      ⌜⟦h__own ∪ h__for⟧ ⇝ log_st⌝.
+
+  Definition lock_inv_ns := nroot.@"lock_inv_ns".
+
+  Definition lock_inv (saddr : socket_address) (γ__lock : gname) (lockv : val)
+                      (i : nat) (st_loc : loc) : iProp Σ :=
+    is_lock lock_inv_ns (ip_of_address saddr) γ__lock lockv (lock_inv_aux i st_loc).
+
+End LockInvariant.
